Add backendTheory, defining the whole backend.
Replaces the _to_target theories. Adds a top-level backend config
record. Compilers for each intermediate language are easily defined from
here (but not currently included).

A few changes made to the interfaces of some parts of the compiler along
the way. The definition of the compiler may still be wrong; indeed, I
think I noticed (and fixed) some problems regarding how the config
parameters are used. It's possible that some config parameters should
instead be hard-coded in the compiler interface (i.e., are not really
configurable).

compiler/backend/clos_to_targetScript.sml
@@ -18,7 +18,7 @@ val compile_def = Define`
   (* TODO: let (exp,calls) = call_intro es in *)
   let (es,l) = remove es in
   let es = annotate es in
-  let (es,aux) = clos_to_bvl$compile es [] in
+  let (es,aux) = clos_to_bvl$compile_exps es [] in
     OPTION_MAP
       (λ(bytes,c). (bytes,(next_loc,c)))
       (bvl_to_target$compile 0 c ((MAP (λe. (0,0,e)) es)++aux))`;
