compiler/backend/exh_to_targetScript.sml
@@ -1,9 +1,0 @@
-open preamble exh_to_patTheory pat_to_targetTheory
-
-val _ = new_theory"exh_to_target";
-
-val compile_def = Define`
-  compile c e =
-    pat_to_target$compile c (exh_to_pat$compile_exp [] e)`;
-
-val _ = export_theory()
