compiler/backend/stack_to_labScript.sml
@@ -1,4 +1,5 @@
 open preamble stackLangTheory labLangTheory;
+local open stack_removeTheory stack_namesTheory in (* stack-to-stack transformations *) end
 
 val _ = new_theory "stack_to_lab";
 
@@ -71,7 +72,58 @@ val flatten_def = Define `
 val prog_to_section_def = Define `
   prog_to_section (n,p) = Section n (FST (flatten p n (max_lab p)))`
 
+val move_inst_def = Define `
+  move_inst dest src =
+    if dest = src then Skip else
+      Seq (Inst (Const dest 0w))
+          (Inst (Arith (Binop Or dest dest (Reg src))))`
+
+val sub_inst_def = Define `
+  sub_inst r1 r2 =
+    Inst (Arith (Binop Sub r1 r1 (Reg r2)))`
+
+val const_inst_def = Define `
+  const_inst r1 w =
+    Inst (Const r1 w)`
+
+val seq_list_def = Define `
+  (seq_list [] = Skip) /\
+  (seq_list [x] = x) /\
+  (seq_list (x::xs) = Seq x (seq_list xs))`
+
+val stub0_def = Define `
+  stub0 sp bp =
+    (0:num, seq_list [move_inst bp 3; (* init base pointer *)
+                      move_inst sp 4; (* init stack pointer *)
+                      move_inst 0 sp;
+                      sub_inst 0 bp;
+                      const_inst 4 (word_offset store_length);
+                      sub_inst 3 4;
+                      (* stack length in 0,
+                         first program point in 1,
+                         heap start is in 2,
+                         heap end is in 3 *)
+                      Call NONE (INL 1) NONE])`;
+
+val stub1_def = Define `
+  stub1 (start:num) =
+    (1:num, seq_list [Set Handler 0;
+                      Set ProgStart 1;
+                      Set CurrHeap 2;
+                      Set LastFree 3;
+                      Call NONE (INL start) NONE])`
+
+val _ = Datatype`config =
+  <| reg_names : num num_map
+   ; stack_ptr : num
+   ; base_ptr : num
+   |>`;
+
 val compile_def = Define `
-  compile prog = MAP prog_to_section prog`;
+  compile start c prog =
+    let prog' = stub1 start :: prog in
+    let without_stack = stub0 c.stack_ptr c.base_ptr :: stack_remove$compile (c.stack_ptr,c.base_ptr) prog' in
+    let with_target_names = stack_names$compile c.reg_names without_stack in
+    MAP prog_to_section with_target_names`;
 
 val _ = export_theory();
