compiler/backend/proofs/word_to_stackProofScript.sml
@@ -268,7 +268,7 @@ val state_rel_def = Define `
     (s.store = t.store \\ Handler) /\ gc_fun_ok t.gc_fun /\
     (!n ignore word_prog arg_count.
        (lookup n s.code = SOME (ignore,word_prog,arg_count)) ==>
-       (lookup n t.code = SOME (word_to_stack$compile word_prog arg_count k))) /\
+       (lookup n t.code = SOME (word_to_stack$compile_prog word_prog arg_count k))) /\
     (lookup 0 t.code = SOME (raise_stub k)) /\ 8 <= dimindex (:'a) /\
     t.stack_space + f <= LENGTH t.stack /\
     (if f' = 0 then f = 0 else (f = f' + f' DIV (dimindex (:'a) - 1) + 1)) /\
